generalized version of Loopfree.v

src/Loopfree.v
@@ -1,48 +1,37 @@
 Require Import CpdtTactics.
+Require Import Closures.
 
-Set Implicit Arguments.
-Load Closures.
+Section CountersImplyLoopfree.
 
-Inductive myprog :=
-  | PHalt
-  | PNext (cont: nat->myprog).
+Variable STATE: Type.
+Variable STEP: STATE -> STATE -> Prop.
+Variable COUNTER: STATE -> nat.
+Variable INCR: forall a b, STEP a b -> COUNTER a < COUNTER b.
 
-Record state := St {
-  StProg: myprog;
-  StVal: nat;
-  StCount: nat }.
+Hint Resolve INCR.
 
-Inductive step: state -> state -> Prop :=
-  | Halt: forall v c, step (St PHalt v c) (St PHalt v (S c))
-  | Next: forall v c cont, step (St (PNext cont) v c) (St (cont v) (S v) (S c)).
-
-Lemma counter_increment:
-  forall a b,
-  step a b -> StCount a < StCount b.
-Proof.
-  intros.  inversion H; crush.
-Qed.
+Ltac clear_step := match goal with
+  | [ H: STEP ?a ?b |- _ ] => assert (COUNTER a < COUNTER b); [ crush | clear H ]; []
+  end.
 
 Lemma counter_monotonic:
   forall a b,
-  star step a b -> StCount a <= StCount b.
+  star STEP a b -> COUNTER a <= COUNTER b.
 Proof.
-  intros.
-  induction H.
-  - crush.
-  - cut (StCount s1 < StCount s2).  crush.  apply counter_increment; crush.
+  induction 1; repeat clear_step; crush.
+Qed.
+Hint Resolve counter_monotonic.
+
+Ltac clear_star_step :=
+  match goal with
+  | [ H: star STEP ?a ?b |- _ ] => assert (COUNTER a <= COUNTER b); [ crush | clear H]; []
+  end.
+
+Theorem star_step_loopfree:
+  forall a b,
+  star STEP a b -> star STEP b a -> a = b.
+Proof.
+  inversion 1; inversion 1; repeat clear_step; repeat clear_star_step; crush.
 Qed.
 
-Theorem step_loopfree:
-  forall a b, star step a b -> star step b a -> a = b.
-Proof.
-  intros.  inversion H; clear H; inversion H0; clear H0.
-  - auto.
-  - assert (StCount b < StCount s2); [ apply counter_increment | idtac ]; crush.
-  - assert (StCount a < StCount s2); [ apply counter_increment | idtac ]; crush.
-  - assert (StCount a < StCount s2); [ apply counter_increment; crush | idtac ].
-    assert (StCount s2 <= StCount b); [ apply counter_monotonic; crush | idtac ].
-    assert (StCount b < StCount s4); [ apply counter_increment; crush | idtac ].
-    assert (StCount s4 <= StCount a); [ apply counter_monotonic; crush | idtac ].
-    crush.
-Qed.
+End CountersImplyLoopfree.
